\begin{enumerate}
	\item On a
	\[
		\begin{aligned}
			\sum_{1\leqslant i \leqslant i \leqslant n} ij 
			&= \sum_{j=1}^n j\left(\sum_{i = 1}^n i\right) \\
			&=  \sum_{j=1}^n ja_j \\
			&=  \sum_{j=1}^n j\frac{j(j+1)}{2} \\
			&= \frac 12 \sum_{j=1}^n j^3 +j^2 \\
			&= \frac{b_n+c_n}{2}\\
			&= \frac{n(n+1)(n+2)(3n+1)}{24}.
		\end{aligned}
	\]
	 \item Posons, pour $i$ fixé, $S_i = \sum_{j=1}^n \min(i,j)$ et commençons par calculer la valeur de $S_i$. Alors, on a
	 \[ S_i = \sum_{j=1}^n j + \sum_{j=i+1}^n i = \frac{i(i+1)}{2} + (n-i)i = \left( n + \frac{1}{2} \right)i - \frac{i^2}{2}.\]
	 On en déduit
	\[
		\begin{aligned}
			 \sum_{i=1}^n \sum_{j=1}^n \min(i,j)
			&= \sum_{i=1}^n S_i \\
			&=  \sum_{i=1}^n \left( n + \frac{1}{2} \right)i - \frac{i^2}{2} \\
			&=  \left( n + \frac{1}{2} \right)\frac{n(n+1)}{2} - \frac{n(n+1)(2n+1)}{12} \\
			&= \frac{n(n+1)(2n+1)}{6}.
		\end{aligned}
	\]
\end{enumerate}